Dependent types would be nice right about now

Invariants.thy
@@ -1,24 +1,30 @@
 theory Invariants
-  imports Main Types HOL.Nat
+  imports Main Types Unsigned Config HOL.Nat
 begin
-
-primrec u64_to_nat :: "u64 \<Rightarrow> nat" where
-  "u64_to_nat (u64 n) = n"
-
-definition valid_u64 :: "u64 \<Rightarrow> bool" where
-  "valid_u64 n \<equiv> u64_to_nat n < 2 ^ 64"
 
 primrec list_len :: "'a List \<Rightarrow> u64" where
   "list_len (List l) = u64 (length l)"
 
-definition valid_list :: "u64 \<Rightarrow> 'a List \<Rightarrow> bool" where
-  "valid_list n l \<equiv> valid_u64 n \<and> u64_to_nat (list_len l) \<le> u64_to_nat n"
+primrec list_inner :: "'a List \<Rightarrow> 'a list" where
+  "list_inner (List l) = l"
+
+definition valid_list :: "('a \<Rightarrow> bool) \<Rightarrow> u64 \<Rightarrow> 'a List \<Rightarrow> bool" where
+  "valid_list pred n l \<equiv>
+    valid_u64 n \<and>
+    u64_to_nat (list_len l) \<le> u64_to_nat n \<and>
+    list_all pred (list_inner l)"
 
 primrec vector_len :: "'a Vector \<Rightarrow> u64" where
   "vector_len (Vector l) = u64 (length l)"
 
-definition valid_vector :: "u64 \<Rightarrow> 'a Vector \<Rightarrow> bool" where
-  "valid_vector n v \<equiv> valid_u64 n \<and> u64_to_nat (vector_len v) = u64_to_nat n"
+primrec vector_inner :: "'a Vector \<Rightarrow> 'a list" where
+  "vector_inner (Vector l) = l"
+
+definition valid_vector :: "('a \<Rightarrow> bool) \<Rightarrow> u64 \<Rightarrow> 'a Vector \<Rightarrow> bool" where
+  "valid_vector pred n v \<equiv>
+    valid_u64 n \<and>
+    u64_to_nat (vector_len v) = u64_to_nat n \<and>
+    list_all pred (vector_inner v)"
 
 primrec slot_to_u64 :: "Slot \<Rightarrow> u64" where
   "slot_to_u64 (Slot n) = n"
@@ -34,6 +40,9 @@ definition valid_epoch :: "Epoch \<Rightarrow> bool" where
 
 definition valid_hash256 :: "Hash256 \<Rightarrow> bool" where
   "valid_hash256 h \<equiv> case h of (Hash256 bytes) \<Rightarrow> length bytes = 32"
+
+definition valid_public_key :: "PublicKey \<Rightarrow> bool" where
+  "valid_public_key k \<equiv> case k of (PublicKey bytes) \<Rightarrow> length bytes = 96"
 
 definition valid_version :: "Version \<Rightarrow> bool" where
   "valid_version v \<equiv> case v of (Version bytes) \<Rightarrow> length bytes = 4"
@@ -52,11 +61,56 @@ definition valid_beacon_block_header :: "BeaconBlockHeader \<Rightarrow> bool" w
     valid_hash256 (state_root header) \<and>
     valid_hash256 (body_root header)"
 
-definition valid_beacon_state :: "BeaconState \<Rightarrow> bool" where
-  "valid_beacon_state state \<equiv>
+definition valid_eth1_data :: "Eth1Data \<Rightarrow> bool" where
+  "valid_eth1_data data \<equiv>
+    valid_hash256 (deposit_root data) \<and>
+    valid_u64 (deposit_count data) \<and>
+    valid_hash256 (block_hash data)"
+
+definition valid_validator :: "Validator \<Rightarrow> bool" where
+  "valid_validator v \<equiv>
+    valid_public_key (pubkey v) \<and>
+    valid_hash256 (withdrawal_credentials v) \<and>
+    valid_u64 (effective_balance v) \<and>
+    valid_epoch (activation_eligibility_epoch v) \<and>
+    valid_epoch (activation_epoch v) \<and>
+    valid_epoch (exit_epoch v) \<and>
+    valid_epoch (withdrawable_epoch v)"
+
+definition valid_bitvector :: "u64 \<Rightarrow> Bitvector \<Rightarrow> bool" where
+  "valid_bitvector n v \<equiv> case v of Bitvector bools \<Rightarrow> length bools = u64_to_nat n"
+
+definition valid_checkpoint :: "Checkpoint \<Rightarrow> bool" where
+  "valid_checkpoint c \<equiv> valid_epoch (Checkpoint.epoch c) \<and> valid_hash256 (Checkpoint.root c)"
+
+definition valid_sync_committee :: "Config \<Rightarrow> SyncCommittee \<Rightarrow> bool" where
+  "valid_sync_committee c sync_committee \<equiv>
+    valid_vector valid_public_key (SYNC_COMMITTEE_SIZE c) (pubkeys sync_committee) \<and>
+    valid_public_key (aggregate_pubkey sync_committee)"
+
+definition valid_beacon_state :: "Config \<Rightarrow> BeaconState \<Rightarrow> bool" where
+  "valid_beacon_state c state \<equiv>
     valid_u64 (genesis_time state) \<and>
     valid_hash256 (genesis_validators_root state) \<and>
     valid_slot (slot state) \<and>
     valid_fork (fork state) \<and>
-    valid_beacon_block_header (latest_block_header state)"
+    valid_beacon_block_header (latest_block_header state) \<and>
+    valid_vector valid_hash256 (SLOTS_PER_HISTORICAL_ROOT c) (block_roots state) \<and>
+    valid_vector valid_hash256 (SLOTS_PER_HISTORICAL_ROOT c) (state_roots state) \<and>
+    valid_list valid_hash256 (HISTORICAL_ROOTS_LIMIT c) (historical_roots state) \<and>
+    valid_eth1_data (eth1_data state) \<and>
+    valid_list valid_eth1_data (SLOTS_PER_ETH1_VOTING_PERIOD c) (eth1_data_votes state) \<and>
+    valid_u64 (eth1_deposit_index state) \<and>
+    valid_list valid_validator (VALIDATOR_REGISTRY_LIMIT c) (validators state) \<and>
+    valid_list valid_u64 (VALIDATOR_REGISTRY_LIMIT c) (balances state) \<and>
+    valid_vector valid_hash256 (EPOCHS_PER_HISTORICAL_VECTOR c) (randao_mixes state) \<and>
+    valid_vector valid_u64 (EPOCHS_PER_SLASHINGS_VECTOR c) (slashings state) \<and>
+    valid_bitvector (JUSTIFICATION_BITS_LENGTH c) (justification_bits state) \<and>
+    valid_checkpoint (previous_justified_checkpoint state) \<and>
+    valid_checkpoint (current_justified_checkpoint state) \<and>
+    valid_checkpoint (finalized_checkpoint state) \<and>
+    valid_list valid_u64 (VALIDATOR_REGISTRY_LIMIT c) (inactivity_scores state) \<and>
+    valid_sync_committee c (current_sync_committee state) \<and>
+    valid_sync_committee c (next_sync_committee state)"
+
 end
