Unsigned.thy
@@ -1,0 +1,57 @@
+theory Unsigned
+  imports Main HOL.Nat
+begin
+
+datatype u8 = u8 nat
+datatype u64 = u64 nat
+
+primrec u64_to_nat :: "u64 \<Rightarrow> nat" where
+  "u64_to_nat (u64 n) = n"
+
+definition valid_u64 :: "u64 \<Rightarrow> bool" where
+  "valid_u64 n \<equiv> u64_to_nat n < 2 ^ 64"
+
+definition check_bin_op ::
+  "('a \<Rightarrow> 'b) \<Rightarrow>
+   ('b \<Rightarrow> 'a) \<Rightarrow>
+   ('a \<Rightarrow> bool) \<Rightarrow>
+   ('b \<Rightarrow> 'b \<Rightarrow> 'b) \<Rightarrow>
+   'a \<Rightarrow> 'a \<Rightarrow> 'a option" where
+  "check_bin_op unwrap wrap check op x y \<equiv>
+    let result = wrap (op (unwrap x) (unwrap y)) in
+    if check result then Some result else None"
+
+definition u64_add :: "u64 \<Rightarrow> u64 \<Rightarrow> u64 option" (infixl ".+" 65) where
+  "u64_add x y \<equiv> check_bin_op u64_to_nat u64 valid_u64 (+) x y"
+
+definition u64_sub :: "u64 \<Rightarrow> u64 \<Rightarrow> u64 option" (infixl ".-" 65) where
+  "u64_sub x y \<equiv>
+    if u64_to_nat x \<ge> u64_to_nat y then
+      check_bin_op u64_to_nat u64 valid_u64 (-) x y
+    else
+      None"
+
+definition u64_mul :: "u64 \<Rightarrow> u64 \<Rightarrow> u64 option" (infixl ".*" 70) where
+  "u64_mul x y \<equiv> check_bin_op u64_to_nat u64 valid_u64 (*) x y"
+
+definition u64_div :: "u64 \<Rightarrow> u64 \<Rightarrow> u64 option" (infixl "\\" 70) where
+  "u64_div x y \<equiv>
+    if y = u64 0 then
+      None
+    else
+      check_bin_op u64_to_nat u64 valid_u64 ((div)) x y"
+
+(* Sanity check lemmas *)
+lemma u64_add_overflow_int_max: "u64 (2 ^ 64 - 1) .+ u64 1 = None"
+  by (clarsimp simp: u64_add_def valid_u64_def check_bin_op_def)
+
+lemma u64_add_overflow_contradiction: "(u64 (2 ^ 64 - 1) .+ u64 1 = Some (u64 0)) \<Longrightarrow> False"
+  by (clarsimp simp: u64_add_def valid_u64_def check_bin_op_def)
+
+lemma u64_sub_overflow_zero: "u64 0 .- u64 1 = None"
+  by (clarsimp simp: u64_sub_def valid_u64_def check_bin_op_def)
+
+lemma u64_div_zero: "n \\ u64 0 = None"
+  by (clarsimp simp: u64_div_def valid_u64_def check_bin_op_def)
+
+end
